running sieve several times in a loop, and only printing the max prime each time. 0-10000 didn't finish even after several seconds and 300+MB memory 0-1000 finished quickly
Also, first 10000 primes finishes quickly.

examples/low-level/SST.ml
@@ -7,7 +7,7 @@ let memread = (fun ( r ) -> !r )
 
 let memwrite = (fun ( r ) ( v ) -> r := v )
 
-let pushStackFrame = (fun ( _ ) -> Camlstack.push_frame 100)
+let pushStackFrame = (fun ( _ ) -> Camlstack.push_frame 100000)
 
 let popStackFrame = (fun ( _ ) -> Camlstack.pop_frame)
 
